## Distributed Network

### P2

d = d_1 + d_2

= (N + P - 1) * (L / R)

The delay of the first packet is N \* (L / R), while the sum delay of the other packets is (P - 1) \* (L / R). So, the result is (N + P - 1) \* (L / R).

### P6

#### question a 

d_drop = m / s sec

#### question b

d_trans = L / R sec

#### question c

d_end-to-end

=d_drop + d_trans

=m / s + L / R

#### question d

The bit just leaves Host A.

#### question e

The bit has not reached Host B but is in the transmission.

#### question f

The bit reached Host B.

#### question g

m = (L \* s) / R

= 536km

### P7

56 * 8 / 64 msec + 56 * 8 / (2 * 1000) msec + 10 msec

= 7 msec + 0.224 msec + 10 msec

= 17.224 msec
